src/pass/mod.rs
@@ -3,6 +3,7 @@ pub mod decay;
 pub mod elab;
 pub mod elim_cis;
 pub mod emit;
+pub mod emit_palow;
 pub mod merge;
 pub mod normalize_casts;
 pub mod prune;
