Makefile
@@ -13,13 +13,17 @@ lib:
 -testsuite: rust lib
 	$(MAKE) -C test
 
+.PHONY: palow-check
+palow-check: rust lib
+	./test/palow-check.sh
+
 .PHONY: format-check
 format-check:
 	cargo fmt --check
 	clang-format --dry-run --Werror cpp/impl.cpp
 
 .PHONY: test
-test: rust lib -testsuite
+test: rust lib -testsuite palow-check
 # Only run formatting checks when tests succeed
 	$(MAKE) format-check
 
